theories/Structures/MonadExc.v
@@ -1,8 +1,10 @@
+From ExtLib.Core Require Import Universes.
 Require Import ExtLib.Structures.Monad.
 
-Class MonadExc (E : Type) (m : Type -> Type) : Type :=
-{ raise : forall {T}, E -> m T
-; catch : forall {T}, m T -> (E -> m T) -> m T
+Class MonadExc@{c d e | c < Universes.u_std, d < Universes.u_std, e < Universes.u_std}
+  (E : Type@{e}) (m : Type@{d} -> Type@{c}) : Type@{max(c, e, d + 1)} :=
+{ raise : forall {T : Type@{d}}, E -> m T
+; catch : forall {T : Type@{d}}, m T -> (E -> m T) -> m T
 }.
 
 Arguments raise {E m mE} {_} _ : rename.
