theories/Core/Universes.v
@@ -1,0 +1,18 @@
+From Coq Require Lists.List.
+
+
+Universe u_list.
+Universe u_std.
+
+Module ConstraintStdUniv.
+  Definition split'@{u_test} (A B : Type@{u_list}) : list (A * B) -> list A * list B :=
+    @Coq.Lists.List.split A B.
+End ConstraintStdUniv.
+
+Constraint u_std < u_list.
+Constraint u_std < Datatypes.list.u0.
+Constraint u_std < Datatypes.sum.u0.
+Constraint u_std < Datatypes.sum.u1.
+Constraint u_std < Datatypes.prod.u0.
+Constraint u_std < Datatypes.prod.u1.
+Constraint u_std < Datatypes.option.u0.
